Begin the weakening lemma
For this it was necessary to introduce a new definition with its set of
lemmas, which is the update_tail.
Reading the paper I noticed that somethimes they introduce variables to
the context by the left, and sometimes by the right. For this lemma it is
introduced by the right.

In practice, variables introduced in the right will not shadow variables
already defined in the context. Whereas variables introduced in the left
will.

src/Coq/SfLib.v
@@ -84,12 +84,33 @@ Definition update {A:Set} (m : partial_map A)
 (x : id) (v : A) :=
 fun x' => if beq_id x x' then (Some v) else m x'.
 
+Print fold_left.
+
+
+Definition update_tail {A:Set} (m : partial_map A) (x : id) (v : A) :=
+fun x' => 
+    match m x' with
+     | None => if beq_id x x' then Some v else None
+     | otherwise => m x'
+    end.
+(*
+if m x' = None 
+
+beq_id x x' then (Some v) else m x'.
+fold_left (fun m u => match u with (x', v') => update empty x' v' end)  [(x, v)] m.
+
+
+Definition update_tail {A:Set} (m : partial_map A) (x : id) (v : A) :=
+fold_left (fun m u => match u with (x', v') => update empty x' v' end)  [(x, v)] m.
+*)
+
 Lemma update_eq : forall A (m: partial_map A) x v,
 (update m x v) x = Some v.
 Proof.
 intros. unfold update. rewrite <- beq_id_refl with (i:= x).
 reflexivity.
 Qed.
+
 
 Theorem update_neq : forall (X:Set) v x1 x2
 (m : partial_map X),
@@ -101,10 +122,30 @@ unfold update. rewrite not_eq_beq_id_false. reflexivity.
 apply H. Qed.
 
 Lemma update_shadow : forall A (m: partial_map A) v1 v2 x,
-update (update m x v1) x v2 = update m x v2.
+(update (update m x v1) x v2) x = Some v2.
 Proof.
-intros A m v1 v2 x1. unfold update.
-Admitted.
+intros A m v1 v2 x.
+unfold update.
+rewrite <- beq_id_refl; auto.
+Qed.
+
+Lemma update_tail_not_shadow : forall A (m: partial_map A) v1 v2 x,
+m x = Some v1 ->
+(update_tail m x v2) x = Some v1.
+Proof.
+intros A m v1 v2 x1 H. unfold update_tail.
+rewrite H; auto.
+Qed.
+
+Lemma update_tail_neq : forall A (m: partial_map A) v x x0,
+x <> x0 ->
+(update_tail m x v) x0 = m x0.
+Proof.
+intros A m v x1 x2 H. unfold update_tail.
+case (m x2). auto.
+rewrite not_eq_beq_id_false; auto.
+
+Qed.
 
 Theorem update_same : forall X v x (m : partial_map X),
 m x = Some v -> 
